working/composition/event_based_refinement/load_balancer/compositional/server/Network.v.dfy
@@ -1,6 +1,6 @@
-include "ServerSpec.t.dfy"
+include "ServerHost.v.dfy"
 include "../shared/Network.t.dfy"
 
 module ServerNetwork refines AbstractNetwork {
-    datatype Message = ServerRequest(request: ServiceRequest<(int, int)>) | ServerResponse(response: ServiceResponse<int>)
+    import opened Host = ServerHost
 }
