working/composition/event_based_refinement/load_balancer/compositional/shared/DistributedSystem.t.dfy
@@ -1,56 +1,57 @@
 include "Types.t.dfy"
 include "Host.t.dfy"
+include "Network.t.dfy"
 
 abstract module AbstractDistributedSystem {
     import opened Types
-    import opened Host: AbstractHost
+    import Network : AbstractNetwork
 
     datatype Constants = Constants(
-        hosts: seq<Host.Constants>,
+        hosts: seq<Network.Host.Constants>,
         network: Network.Constants) 
     {
         ghost predicate WF() 
         {
-            Host.GroupWFConstants(hosts)
+            Network.Host.GroupWFConstants(hosts)
         }
     }
 
     datatype Variables = Variables(
-        hosts: seq<Host.Variables>,
+        hosts: seq<Network.Host.Variables>,
         network: Network.Variables) 
     {
         ghost predicate WF(c: Constants) {
             && c.WF()
             && |c.hosts| == |hosts|
-            && Host.GroupWFVariables(c.hosts, hosts)
+            && Network.Host.GroupWFVariables(c.hosts, hosts)
         }
     }
 
     ghost predicate Init(c: Constants, v: Variables) {
         && v.WF(c)
-        && (forall i :: 0 <= i < |c.hosts| ==> Host.Init(c.hosts[i], v.hosts[i]))
+        && (forall i :: 0 <= i < |c.hosts| ==> Network.Host.Init(c.hosts[i], v.hosts[i]))
         && Network.Init(c.network, v.network)
     }
 
-    ghost predicate HostAction(c: Constants, v: Variables, v': Variables, evt: Option<Spec.Event>, hostId: nat, msgOps: Network.MessageOps)
+    ghost predicate HostAction(c: Constants, v: Variables, v': Variables, evt: Option<Network.Host.Spec.Event>, hostId: nat, msgOps: Network.Host.MessageOps)
     {
         && v.WF(c)
         && v'.WF(c)
         && 0 <= hostId < |v.hosts|
-        && Host.Next(c.hosts[hostId], v.hosts[hostId], v'.hosts[hostId], evt, msgOps)
+        && Network.Host.Next(c.hosts[hostId], v.hosts[hostId], v'.hosts[hostId], evt, msgOps)
         && (forall i :: 0 <= i < |v.hosts| && i != hostId ==> v.hosts[i] == v'.hosts[i])
         && Network.Next(c.network, v.network, v'.network, msgOps)
     }
 
     datatype Step =
-        | HostActionStep(hostId: nat, msgOps: Network.MessageOps)
+        | HostActionStep(hostId: nat, msgOps: Network.Host.MessageOps)
 
-    ghost predicate NextStep(c: Constants, v: Variables, v': Variables, evt: Option<Spec.Event>, step: Step)
+    ghost predicate NextStep(c: Constants, v: Variables, v': Variables, evt: Option<Network.Host.Spec.Event>, step: Step)
     {
         && HostAction(c, v, v', evt, step.hostId, step.msgOps)
     }
 
-    ghost predicate Next(c: Constants, v: Variables, v': Variables, evt: Option<Spec.Event>)
+    ghost predicate Next(c: Constants, v: Variables, v': Variables, evt: Option<Network.Host.Spec.Event>)
     //{
     //    exists step :: NextStep(c, v, v', evt, step)
     //}
