working/composition/event_based_refinement/load_balancer/compositional/shared/Host.t.dfy
@@ -1,11 +1,12 @@
 include "Types.t.dfy"
 include "Spec.t.dfy"
-include "Network.t.dfy"
 
 abstract module AbstractHost {
     import opened Types
     import opened Spec: AbstractSpec
-    import Network: AbstractNetwork
+
+    type Message(==)
+    datatype MessageOps = MessageOps(recv:Option<Message>, send:Option<Message>)
 
     type Constants {
         ghost predicate WF()
@@ -19,5 +20,5 @@ abstract module AbstractHost {
     ghost predicate GroupWFVariables(c: seq<Constants>, v: seq<Variables>)
 
     ghost predicate Init(c: Constants, v: Variables)
-    ghost predicate Next(c: Constants, v: Variables, v': Variables, evt: Option<Spec.Event>, msgOps: Network.MessageOps)
+    ghost predicate Next(c: Constants, v: Variables, v': Variables, evt: Option<Spec.Event>, msgOps: MessageOps)
 }
