working/composition/event_based_refinement/load_balancer/compositional/client_server/ClientServerHost.v.dfy
@@ -1,0 +1,20 @@
+include "../abstract_composition/ComposedHost.t.dfy"
+include "ClientServerSpec.t.dfy"
+
+module ClientServerHost refines ComposedHost {
+    import opened Spec = ClientServerSpec
+
+    ghost predicate TranslateAToB(msgA: HostA.Message, msgB: HostB.Message)
+    {
+        && msgA.ClientRequest?
+        && msgB.ServerRequest?
+        && msgA.request == msgB.request
+    }
+
+    ghost predicate TranslateBToA(msgB: HostB.Message, msgA: HostA.Message)
+    {
+        && msgB.ServerResponse?
+        && msgA.ClientResponse?
+        && msgB.response == msgA.response
+    }
+}
